examples/t2/P25.v
@@ -1,0 +1,107 @@
+
+From CTree Require Import
+  CTree.Core
+  Events.Writer
+  Logic.Ctl
+  CTree.Equ
+  CTree.SBisim
+  CTree.Logic.Trans
+  Logic.Kripke
+  CTree.Interp.Core
+  CTree.Logic.AF
+  CTree.Logic.AX
+  CTree.Logic.Bind
+  CTree.Logic.Iter
+  CTree.Logic.State
+  CTree.Logic.CanStep
+  CTree.Interp.State
+  CTree.Events.State
+  CTree.Events.Writer.
+
+From Coq Require Import
+  ZArith.
+
+Generalizable All Variables.
+
+Import Ctree CTreeNotations CtlNotations.
+Local Open Scope ctree_scope.
+Local Open Scope ctl_scope.
+Local Open Scope Z_scope.
+
+
+(*
+// OK
+// (varC <= 5) || ([AF](varR > 5))
+// -ctl "OR{varC <= 5}{AF{varR > 5}}
+// -joinbwd 6
+
+void main() {
+
+    int varC; // assume varC >= 1
+    int varR = 0;
+    int varCS = 8;
+
+    while (varCS > 0) {
+        if (varC >= varCS) {
+            varC = varC - 1;
+            varR = varR + 1;
+            varCS = varCS - 1;
+        } else {
+            varC = varC - 1; 
+            varR = varR + 1; 
+            varCS = varCS - 1;
+        }
+    }
+
+}
+ *)
+
+Module Clang.
+
+  Record Mem := { varC : Z; varR : Z; varCS: Z }.
+
+  Definition setC (c: Z): ctree (stateE Mem) unit :=
+    m <- get ;;
+    put {| varC := c; varR := m.(varR); varCS := m.(varCS) |}.
+  
+  Definition setR (r: Z): ctree (stateE Mem) unit :=
+    m <- get ;;
+    put {| varC := m.(varC); varR := r; varCS := m.(varCS) |}.
+
+  Definition setCS (cs: Z): ctree (stateE Mem) unit :=
+    m <- get ;;
+    put {| varC := m.(varC); varR := m.(varR); varCS := cs |}.
+
+  Definition p25: ctree (stateE Mem) unit :=
+    setR 0%Z ;;
+    setCS 8%Z ;;
+    iter (fun _ =>
+            m <- get;;
+            if (0%Z <? m.(varCS)) then (
+                   setC (m.(varC) - 1) ;;
+                   setR (m.(varR) + 1) ;;
+                   setCS (m.(varCS) - 1) ;;
+                   continue
+                 )
+            else break) tt.
+
+  (* // (varC <= 5) || ([AF](varR > 5)) *)
+  Lemma p25_spec: forall c r cs,
+      c >= 1%Z ->
+      <( {instr_stateE p25 {| varC := c; varR := r; varCS := cs |} }, Pure |=
+           (visW {fun m => m.(varC) <= 5%Z} \/ AF visW {fun m => m.(varR) > 5}) )>.
+  Proof with eauto with ctl.
+    intros.
+    unfold p25.
+    cright.
+    eapply aul_state_bind_r_eq.
+    - cleft.
+      csplit...
+      + csplit...
+      + eapply can_step_state_bind_l.
+        * unfold get, trigger; rewrite interp_state_vis.
+          cbn; apply ktrans_vis.
+          exists tt; intuition.
+        * constructor.
+      + intros.
+        
