theories/Events/StateE.v
@@ -35,6 +35,7 @@ Section State.
                | Put s' => (tt, s')
                end).
 
+   
 End State.
 
 Arguments Get {S}.
